feat: bv_decide BitVec.sdiv (#5823)

src/Std/Tactic/BVDecide/Bitblast/BVExpr/Basic.lean
@@ -73,6 +73,10 @@ inductive BVBinOp where
   Unsigned modulo.
   -/
   | umod
+  /--
+  Signed division.
+  -/
+  | sdiv
 
 namespace BVBinOp
 
@@ -84,6 +88,7 @@ def toString : BVBinOp → String
   | mul => "*"
   | udiv => "/ᵤ"
   | umod => "%ᵤ"
+  | sdiv => "/ₛ"
 
 instance : ToString BVBinOp := ⟨toString⟩
 
@@ -98,6 +103,7 @@ def eval : BVBinOp → (BitVec w → BitVec w → BitVec w)
   | mul => (· * ·)
   | udiv => (· / ·)
   | umod => (· % · )
+  | sdiv => BitVec.sdiv
 
 @[simp] theorem eval_and : eval .and = ((· &&& ·) : BitVec w → BitVec w → BitVec w) := by rfl
 @[simp] theorem eval_or : eval .or = ((· ||| ·) : BitVec w → BitVec w → BitVec w) := by rfl
@@ -106,6 +112,7 @@ def eval : BVBinOp → (BitVec w → BitVec w → BitVec w)
 @[simp] theorem eval_mul : eval .mul = ((· * ·) : BitVec w → BitVec w → BitVec w) := by rfl
 @[simp] theorem eval_udiv : eval .udiv = ((· / ·) : BitVec w → BitVec w → BitVec w) := by rfl
 @[simp] theorem eval_umod : eval .umod = ((· % ·) : BitVec w → BitVec w → BitVec w) := by rfl
+@[simp] theorem eval_sdiv : eval .sdiv = (BitVec.sdiv : BitVec w → BitVec w → BitVec w) := by rfl
 
 end BVBinOp
 
